src/StAM.v
@@ -4,14 +4,69 @@ Record representing the AM Monad state structure.
 Author:  Adam Petz, ampetz@ku.edu
 *)
 
-Require Import Maps.
+Require Import Maps StructTactics Term.
 Require Import Coq.Arith.EqNat.
 
+Require Import List.
+Import ListNotations.
+
 Definition BS := nat.
+
+Definition eqbPair{A B:Type}`{H:EqClass A}`{H':EqClass B} (p1:A*B) (p2:A*B) : bool :=
+  match (p1,p2) with
+  | ((a1,b1), (a2,b2)) => andb (eqb a1 a2) (eqb b1 b2)
+  end.
+
+Search beq_nat_true.
+Check beq_nat_true.
+
+Lemma beq_pair_true{A B:Type}`{H:EqClass A}`{H':EqClass B} : forall (p1 p2:(A*B)),
+    eqbPair p1 p2 = true -> p1 = p2.
+Proof.
+  intros.
+  unfold eqbPair in *.
+  repeat break_let.
+  assert (a = a0).
+  {
+    assert (eqb a a0 = true).
+    {
+      destruct (eqb a a0); try solve_by_inversion.
+    }
+    Check beq_nat_true.
+    eapply eqb_leibniz; eauto.
+  }
+  
+  assert (b = b0).
+  {
+        assert (eqb b b0 = true).
+        {
+          destruct (eqb b b0); try reflexivity.
+          cbv in *.
+          repeat break_let.
+          break_if; solve_by_inversion.     
+        }
+    eapply eqb_leibniz; eauto.
+  }
+  subst.
+  reflexivity.
+Defined.
+
+                                                             
+
+
+Instance pair_EqClass{A B:Type}`{H:EqClass A}`{H':EqClass B} : EqClass (A*B) :=
+  { eqb:= eqbPair;
+    eqb_leibniz := beq_pair_true }.
+
+Definition asp_map := MapC (Plc * ASP_ID) ASP_ID.
 
 (* Specific AM monad state *)
 Record AM_St : Type := mkAM_St
                          { am_nonceMap : MapC nat BS;
                            am_nonceId : nat;
-                           checked : list nat }.
+                           st_aspmap :asp_map(*;
+                           checked : list nat*) }.
+
+Definition empty_amst :=
+  mkAM_St [] 0 [].
                                          
