src/GenStMonad.v
@@ -51,5 +51,9 @@ Notation "x <- c1 ;; c2" := (@bind _ _ _ c1 (fun x => c2))
 Notation "e1 ;; e2" := (_ <- e1 ;; e2)
                          (at level 100, right associativity).
 
+Definition gets {S} {A} (f:S -> A) : St S A :=
+  st <- get ;;
+  ret (f st).
+
 Definition when {S A} (b : bool) (m : St S A) : St S unit :=
   if b then m ;; ret tt else nop.
