src/StVM.v
@@ -6,6 +6,8 @@ Author:  Adam Petz, ampetz@ku.edu
 
 Require Import ConcreteEvidence.
 Require Import Maps.
+Require Import List.
+Import ListNotations.
 
 (* Specific VM monad state *)
 Definition ev_store := MapC nat EvidenceC.
@@ -14,3 +16,5 @@ Record vm_st : Type := mk_st
                           st_trace:list Ev ;
                           st_pl:Plc ;
                           st_store:ev_store}.
+
+Definition empty_vmst := mk_st mtc [] 0 [].
