src/VM_IO_Axioms.v
@@ -1,0 +1,12 @@
+Require Import Term ConcreteEvidence.
+
+(** IO Axioms *)
+
+Definition parallel_att_vm_thread (t:AnnoTerm) (e:EvidenceC) : EvidenceC.
+Admitted.
+
+Definition parallel_vm_events (t:AnnoTerm) (p:Plc) : list Ev.
+Admitted.
+
+Definition shuffled_events (el1:list Ev) (el2:list Ev) : list Ev.
+Admitted.
