src/VmSemantics.v
@@ -8,7 +8,7 @@ Require Import More_lists Preamble Term ConcreteEvidence LTS GenStMonad.
 Require Import Main Event_system Term_system.
 
 
-Require Import MonadVM MonadVMFacts Maps.
+Require Import MonadVM MonadVMFacts Maps VM_IO_Axioms.
 
 Require Import List.
 Import ListNotations.
@@ -20,16 +20,6 @@ Require Import StructTactics.
 
 Set Nested Proofs Allowed.
 
-(** IO Axioms *)
-
-Definition parallel_att_vm_thread (t:AnnoTerm) (e:EvidenceC) : EvidenceC.
-Admitted.
-
-Definition parallel_vm_events (t:AnnoTerm) (p:Plc) : list Ev.
-Admitted.
-
-Definition shuffled_events (el1:list Ev) (el2:list Ev) : list Ev.
-Admitted.
 
 Fixpoint build_comp (t:AnnoTerm): VM unit :=
   match t with
