src/extra/LtacBug.v
@@ -1,0 +1,36 @@
+Lemma temp{A:Type} : forall (a:A), a = a.
+Proof.
+  trivial.
+Defined.
+
+Set Ltac Debug.
+
+Ltac temp_ltac :=
+  match goal with
+  | [H: ?a = _ |- _] => apply temp with (a:=a); eauto
+  end.
+
+Example temp_ex{A:Type} : forall (c:A), c = c -> c = c.
+Proof.
+  intros.
+  Fail temp_ltac.
+  apply temp with (c:=c).
+  Check temp.
+  eapply temp with (a0:=a).
+​
+Example temp_ex{A:Type} : forall (c:A),  c = c -> c = c.
+Proof.
+
+​
+Ltac temp_ltac' :=
+  match goal with
+  | [H: ?b = _ |- _] => apply temp with (a:=b); eauto
+  end.
+​
+Example temp_ex{A:Type} : forall (c:A),  c = c -> c = c.
+Proof.
+  intros.
+  Fail temp_ltac.
+  (* evaluates to:       apply temp with (c:=c); eauto *)
+  (* should evaluate to: apply temp with (a:=c); eauto *)
+  temp_ltac'.
